Term.v
@@ -90,6 +90,20 @@ Inductive EvidenceC: Set :=
 | ssc: EvidenceC -> EvidenceC -> EvidenceC
 | ppc: EvidenceC -> EvidenceC -> EvidenceC.
 
+(** * Place-holder axioms for IO operations *)
+Definition invokeKIM (i:ASP_ID) (q:Plc) (args:list Arg) : BS.
+Admitted.
+Definition invokeUSM (i:ASP_ID) (args:list Arg) : BS.
+Admitted.
+Definition signEv (e:EvidenceC) : BS.
+Admitted.
+Definition hashEv (e:EvidenceC) : BS.
+Admitted.
+Definition toRemote (t:Term) (pTo:Plc) (e:EvidenceC) : EvidenceC.
+Admitted.
+Definition parallel_eval_thread (t:Term) (e:EvidenceC) : EvidenceC.
+Admitted.
+
 Fixpoint et_fun (p:Plc) (ec:EvidenceC) : Evidence :=
   match ec with
   | mtc => mt
@@ -753,3 +767,49 @@ Proof.
     + events_event_range.
     + events_event_range.
 Qed.
+
+
+(** * Eval function definition *)
+Definition splitEv (sp:SP) (e:EvidenceC) : EvidenceC :=
+  match sp with
+  | ALL => e
+  | NONE => mtc
+  end.
+
+Definition eval_asp (a:ASP) (e:EvidenceC) : EvidenceC :=
+  match a with
+  | CPY => e
+  | KIM i q args =>
+    let bs := invokeKIM i q args in
+    (kkc i args q bs e)
+  | USM i args =>
+    let bs := invokeUSM i args in
+    (uuc i args bs e)
+  | SIG =>
+    let bs := signEv e in
+    (ggc e bs)
+  | HSH =>
+    let bs := hashEv e in
+    (hhc bs e)
+  end.
+
+Fixpoint eval (t:Term) (e:EvidenceC) : EvidenceC :=
+  match t with
+  | asp a => eval_asp a e
+  | att q t1 => toRemote t1 q e
+  | lseq t1 t2 =>
+    let e1 := eval t1 e in
+    eval t2 e1
+  | bseq (sp1,sp2) t1 t2 =>
+    let e1 := splitEv sp1 e in
+    let e2 := splitEv sp2 e in
+    let e1' := eval t1 e1 in
+    let e2' := eval t2 e2 in
+    (ssc e1' e2')
+  | bpar (sp1,sp2) t1 t2 =>
+    let e1 := splitEv sp1 e in
+    let e2 := splitEv sp2 e in
+    let e1' := parallel_eval_thread t1 e1 in
+    let e2' := parallel_eval_thread t2 e2 in
+    (ppc e1' e2')
+  end.
